Whole proof of monadic interpreter starting from run_iter  (#7)
* Hoare triple proof of run_iter

* Grow_memory complete

* Load almost done

* tidying up Load (in Wasm_Interpreter_Monad_Properties.thy)

* tyding up Load (cont.)

* tyding up Load (Byte_Array.thy)

* adding store triples in Byte_Array.thy

* Store proof finished (along with a fix in the interpreter)

* Improve extract_pre_pure

* Organise a bit

* Simplify proofs involving host_apply_impl_m

WebAssembly/Wasm_Interpreter_Monad_Properties.thy
@@ -184,11 +184,8 @@ proof -
     by (simp add: Abs_uint64_inverse map_takefill Abs_uint8'.abs_eq zero_uint8.abs_eq)
 qed
   
-  term app_s_f_v_s_mem_size_m
-term app_s_f_v_s_mem_size
 
-
-definition "mem_m_assn \<equiv> \<lambda>(mr,mm) (mr_m,mm_m). mr_m \<mapsto>\<^sub>b\<^sub>aRep_mem_rep mr * \<up>(mm_m=mm)"
+(* separation logic methods *)
 
 method extract_list_idx for i :: nat =
   (subst listI_assn_extract[of i], (simp;fail), (simp;fail))
@@ -202,9 +199,39 @@ method reinsert_list_idx for i :: nat =
 method knock_down for i :: nat = 
  extract_pre_pure?, extract_list_idx i, sep_auto, extract_pre_pure?, reinsert_list_idx i
 
-term app_s_f_v_s_mem_size_m
-term app_s_f_v_s_mem_size
+lemmas is_complex_goal = asm_rl[of "< _ > _ < _ >"] asm_rl[of "_ \<Longrightarrow>\<^sub>A _"]
 
+method_setup then_else = \<open>let
+in
+  Method.text_closure -- Method.text_closure -- Method.text_closure >>
+    (fn ((textb, textt), texte) => fn ctxt => fn using => fn st =>
+      let
+        val bmethod = Method.evaluate_runtime textb ctxt using;
+        val tmethod = Method.evaluate_runtime textt ctxt using;
+        val emethod = Method.evaluate_runtime texte ctxt using;
+      in
+        (case try (fn st => bmethod st |> Seq.pull) st of
+          SOME (SOME (Seq.Result st,_)) => tmethod st
+        | _ => emethod st)
+      end)
+end     
+\<close>
+
+method defer_vcg = then_else \<open>rule is_complex_goal\<close> \<open>fail\<close> 
+  \<open>find_goal \<open>rule is_complex_goal\<close>, 
+  (rule is_complex_goal | tactic \<open>defer_tac 1\<close>)\<close>
+
+method sep_auto_all = (defer_vcg | (rule is_complex_goal, sep_auto))+
+
+
+
+abbreviation "expect_assn A B x_opt y_opt \<equiv> (case x_opt of 
+  Some x \<Rightarrow> (case y_opt of Some y \<Rightarrow> A x y | None \<Rightarrow> false)
+  | None \<Rightarrow> (case y_opt of Some y \<Rightarrow> false | None \<Rightarrow> B)
+  )"
+
+
+(* assertions *) 
 
 definition "inst_m_assn i i_m \<equiv> 
     inst_m.types i_m \<mapsto>\<^sub>a inst.types i
@@ -213,11 +240,6 @@ definition "inst_m_assn i i_m \<equiv>
   * inst_m.mems  i_m \<mapsto>\<^sub>a inst.mems  i 
   * inst_m.globs i_m \<mapsto>\<^sub>a inst.globs i"
 
-lemma [sep_heap_rules]: "<mem_m_assn m mi> len_byte_array (fst mi) 
-<\<lambda>r. mem_m_assn m mi * \<up>(r=length (Rep_mem_rep (fst m)))>"
-  unfolding mem_m_assn_def
-  by (sep_auto split: prod.splits)
-
 type_synonym inst_store = "(inst list \<times> inst_m list)"
 
 abbreviation "inst_store_assn \<equiv> \<lambda>(is, i_ms). list_assn inst_m_assn is i_ms"
@@ -225,9 +247,6 @@ abbreviation "inst_store_assn \<equiv> \<lambda>(is, i_ms). list_assn inst_m_ass
 abbreviation "inst_at \<equiv> \<lambda>(is, i_ms) (i, i_m) j. j < length is \<and> is!j = i \<and> i_ms!j = i_m"
 
 abbreviation "contains_inst_assn i_s i \<equiv> \<exists>\<^sub>A j. \<up>(inst_at i_s i j)"
-
-definition mems_m_assn :: "mem list \<Rightarrow> mem_m array \<Rightarrow> assn" where
-  "mems_m_assn ms ms_m = (\<exists>\<^sub>A ms_i. ms_m \<mapsto>\<^sub>a ms_i  * list_assn mem_m_assn ms ms_i)"
 
 definition cl_m_assn :: "inst_store \<Rightarrow> cl \<Rightarrow> cl_m \<Rightarrow> assn" where 
   "cl_m_assn i_s cl cl_m = (case cl of 
@@ -242,26 +261,16 @@ definition cl_m_assn :: "inst_store \<Rightarrow> cl \<Rightarrow> cl_m \<Righta
   | cl_m.Func_host tf_m host_m \<Rightarrow> \<up>(tf = tf_m \<and> host = host_m))
 )"
 
-lemma ex_assn_pure_conv:"(\<exists>\<^sub>Ax. \<up>(P x)) = \<up>(\<exists>x. P x)"
-  by (smt (z3) ent_ex_preI ent_iffI ent_pure_pre_iff_sng ent_refl triv_exI)
-
-lemma cl_m_assn_pure:"is_pure_assn (cl_m_assn i_s cl cl_m)"
-  unfolding cl_m_assn_def 
-  by(simp split: cl.split cl_m.split add:ex_assn_pure_conv)
-  
-
-lemma cl_m_assn_type:
-  assumes "h \<Turnstile> cl_m_assn i_s cl cl_m" 
-  shows "cl_type cl = cl_m_type cl_m"
-  using assms
-  unfolding cl_m_assn_def cl_type_def cl_m_type_def
-  by(simp split:cl.splits cl_m.splits)
-
 definition funcs_m_assn :: "inst_store \<Rightarrow> cl list \<Rightarrow> cl_m array \<Rightarrow> assn" where
   "funcs_m_assn i_s fs fs_m = (\<exists>\<^sub>A fs_i. fs_m \<mapsto>\<^sub>a fs_i * list_assn (cl_m_assn i_s) fs fs_i)"
 
 definition tabinst_m_assn :: "tabinst \<Rightarrow> tabinst_m \<Rightarrow> assn" where 
   "tabinst_m_assn = (\<lambda>(tr,tm) (tr_m,tm_m). tr_m \<mapsto>\<^sub>a tr * \<up>(tm = tm_m))"
+
+definition "mem_m_assn \<equiv> \<lambda>(mr,mm) (mr_m,mm_m). mr_m \<mapsto>\<^sub>b\<^sub>aRep_mem_rep mr * \<up>(mm_m=mm)"
+
+definition mems_m_assn :: "mem list \<Rightarrow> mem_m array \<Rightarrow> assn" where
+  "mems_m_assn ms ms_m = (\<exists>\<^sub>A ms_i. ms_m \<mapsto>\<^sub>a ms_i  * list_assn mem_m_assn ms ms_i)"
 
 definition tabs_m_assn :: "tabinst list \<Rightarrow> tabinst_m array \<Rightarrow> assn" where
  "tabs_m_assn ts ts_m = (\<exists>\<^sub>A ts_i. ts_m \<mapsto>\<^sub>a ts_i * list_assn tabinst_m_assn ts ts_i)"
@@ -289,10 +298,6 @@ definition fc_m_assn :: "inst_store \<Rightarrow> frame_context \<Rightarrow> fr
 
 definition "fcs_m_assn i_s fcs fcs_m \<equiv> list_assn (fc_m_assn i_s) fcs fcs_m"
 
-lemma [simp]:"fcs_m_assn i_s (fc#fcs) (fc_m#fcs_m) = 
-  fc_m_assn i_s fc fc_m * fcs_m_assn i_s fcs fcs_m"
-  unfolding fcs_m_assn_def by simp
-
 definition cfg_m_assn :: "inst_store \<Rightarrow> config \<Rightarrow> config_m \<Rightarrow> assn" where
   "cfg_m_assn i_s cfg cfg_m = (
   case cfg of Config d s fc fcs \<Rightarrow>
@@ -301,26 +306,106 @@ definition cfg_m_assn :: "inst_store \<Rightarrow> config \<Rightarrow> config_m
    * inst_store_assn i_s
 )"     
 
+
+
+(*  heap rules, lemmas etc. about the assertions above *)
+
+lemma ex_assn_pure_conv:"(\<exists>\<^sub>Ax. \<up>(P x)) = \<up>(\<exists>x. P x)"
+  by (smt (z3) ent_ex_preI ent_iffI ent_pure_pre_iff_sng ent_refl triv_exI)
+
+lemma cl_m_assn_pure:"is_pure_assn (cl_m_assn i_s cl cl_m)"
+  unfolding cl_m_assn_def 
+  by(simp split: cl.split cl_m.split add:ex_assn_pure_conv)
+
+lemma cl_m_assn_type:
+  assumes "h \<Turnstile> cl_m_assn i_s cl cl_m" 
+  shows "cl_type cl = cl_m_type cl_m"
+  using assms
+  unfolding cl_m_assn_def cl_type_def cl_m_type_def
+  by(simp split:cl.splits cl_m.splits)
+
+lemma pure_dup:
+  assumes "is_pure_assn P" 
+  shows "P = P*P" 
+  using assms unfolding is_pure_assn_def
+  by auto
+
+lemma [sep_heap_rules]: "<tabinst_m_assn t t_m> 
+    Array.len (fst t_m) 
+    <\<lambda>r. tabinst_m_assn t t_m * \<up>(r=length (fst t))>"
+  unfolding tabinst_m_assn_def
+  by (sep_auto split: prod.splits)
+
+lemma [sep_heap_rules]: "<tabinst_m_assn t t_m> 
+    Array.nth (fst t_m) x
+    <\<lambda>r. tabinst_m_assn t t_m * \<up>(r=(fst t)!x)>"
+  unfolding tabinst_m_assn_def
+  by (sep_auto split: prod.splits)
+
+lemma funcs_nth_type_triple:"<funcs_m_assn i_s cls cls_m> 
+    Array.nth cls_m i  
+    <\<lambda>r. \<up>(cl_m_type r = cl_type (cls!i)) * funcs_m_assn i_s cls cls_m>" 
+  unfolding funcs_m_assn_def list_assn_conv_idx
+  apply(sep_auto heap del:nth_rule)
+  apply(extract_pre_pure)
+  apply(sep_auto)
+  apply(simp add: listI_assn_extract[of i])
+  using cl_m_assn_type 
+  by (metis mod_starD)
+
+lemma [sep_heap_rules]: "<mem_m_assn m mi> 
+    len_byte_array (fst mi) 
+    <\<lambda>r. mem_m_assn m mi * \<up>(r=length (Rep_mem_rep (fst m)))>"
+  unfolding mem_m_assn_def
+  by (sep_auto split: prod.splits)
+
+definition "fc_m_assn_pure fc fc_m \<equiv> (
+  case fc of Frame_context redex lcs nf f \<Rightarrow> 
+  case fc_m of Frame_context_m redex_m lcs_m nf_m f_locs1 f_inst2 \<Rightarrow>
+  redex = redex_m \<and> lcs = lcs_m \<and> nf = nf_m)"
+
+lemma extract_pre_fc_m_assn[extract_pure_rules]: 
+  "h \<Turnstile> fc_m_assn i_s fc fc_m \<Longrightarrow> fc_m_assn_pure fc fc_m"
+  unfolding fc_m_assn_def fc_m_assn_pure_def 
+  by (sep_auto split:frame_context.splits frame_context_m.splits)
+
+lemma [simp]:"fcs_m_assn i_s (fc#fcs) (fc_m#fcs_m) = 
+  fc_m_assn i_s fc fc_m * fcs_m_assn i_s fcs fcs_m"
+  unfolding fcs_m_assn_def by simp
+
+definition "cfg_m_assn_pure cfg cfg_m = (
+  case cfg of Config d s fc fcs \<Rightarrow>
+  case cfg_m of Config_m d_m s_m fc_m fcs_m \<Rightarrow> 
+  d=d_m \<and> fc_m_assn_pure fc fc_m \<and> length fcs = length fcs_m
+)"     
+
+lemma extract_pre_cfg_m_assn[extract_pure_rules]: 
+  "h \<Turnstile> cfg_m_assn i_s cfg cfg_m \<Longrightarrow> cfg_m_assn_pure cfg cfg_m"
+  unfolding cfg_m_assn_def cfg_m_assn_pure_def fcs_m_assn_def
+  apply (sep_auto split:config.splits config_m.splits)
+  subgoal by (metis mod_starE extract_pre_fc_m_assn)
+  by (metis mod_starE extract_pre_list_assn_lengthD) 
+   
+
+(* hoare triples for run_step_b_e_m *)
+
 lemma mem_size_triple:
   assumes "inst_at (is, i_ms) (f_inst f, f_inst2) j" 
   shows 
-  "< ms_m \<mapsto>\<^sub>a ms_i * list_assn mem_m_assn ms ms_i * inst_store_assn (is, i_ms) > 
+  "< mems_m_assn ms ms_m * inst_store_assn (is, i_ms) > 
     app_s_f_v_s_mem_size_m ms_m f_inst2 v_s 
   <\<lambda>r. \<up>(r = app_s_f_v_s_mem_size ms f v_s) *
-   ms_m \<mapsto>\<^sub>a ms_i * (list_assn mem_m_assn) ms ms_i * inst_store_assn (is, i_ms)>"
+   mems_m_assn ms ms_m * inst_store_assn (is, i_ms)>"
   using assms
-  unfolding app_s_f_v_s_mem_size_m_def inst_m_assn_def list_assn_conv_idx
+  unfolding app_s_f_v_s_mem_size_m_def inst_m_assn_def mems_m_assn_def list_assn_conv_idx
   apply sep_auto
    apply (knock_down j)
   apply(sep_auto)
   apply(knock_down "inst.mems (f_inst f) ! 0")
    apply (sep_auto)
-  subgoal by (auto simp add: app_s_f_v_s_mem_size_def smem_ind_def mem_size_def 
+  apply (auto simp add: app_s_f_v_s_mem_size_def smem_ind_def mem_size_def 
         mem_length_def mem_rep_length_def split: option.split list.split)  
-  apply (sep_auto)
   done
-
-
 
 lemma get_local_triple: 
   "<locs_m_assn (f_locs f) f_locs1> 
@@ -328,7 +413,6 @@ lemma get_local_triple:
   <\<lambda>r. \<up>(r = app_f_v_s_get_local k f v_s) * locs_m_assn (f_locs f) f_locs1>"
   unfolding locs_m_assn_def app_f_v_s_get_local_m_def app_f_v_s_get_local_def
   by sep_auto
-
 
 lemma get_global_triple:
   assumes "inst_at (is, i_ms) (f_inst f, f_inst2) j"
@@ -355,7 +439,6 @@ lemma set_local_triple:
   unfolding locs_m_assn_def app_f_v_s_set_local_m_def app_f_v_s_set_local_def
   by(sep_auto)
 
-
 (*unfortunately I have to phrase it as (is, i_ms), otherwise sep_auto gets confused*)
 lemma set_global_triple: 
   assumes "inst_at (is, i_ms) (f_inst f, f_inst2) j"
@@ -372,9 +455,6 @@ lemma set_global_triple:
   apply(sep_auto)
   done
 
-
-(* app_s_f_v_s_set_global_def update_glob_def sglob_ind_def Let_def *)
-
 lemma call_triple: 
   assumes "inst_at (is, i_ms) (f_inst f, f_inst2) j"
   shows
@@ -387,54 +467,6 @@ lemma call_triple:
    apply(knock_down j)
   apply(sep_auto)
   done
-
-
-lemmas is_complex_goal = asm_rl[of "< _ > _ < _ >"] asm_rl[of "_ \<Longrightarrow>\<^sub>A _"]
-
-method_setup then_else = \<open>let
-in
-  Method.text_closure -- Method.text_closure -- Method.text_closure >>
-    (fn ((textb, textt), texte) => fn ctxt => fn using => fn st =>
-      let
-        val bmethod = Method.evaluate_runtime textb ctxt using;
-        val tmethod = Method.evaluate_runtime textt ctxt using;
-        val emethod = Method.evaluate_runtime texte ctxt using;
-      in
-        (case try (fn st => bmethod st |> Seq.pull) st of
-          SOME (SOME (Seq.Result st,_)) => tmethod st
-        | _ => emethod st)
-      end)
-end     
-\<close>
-
-method defer_vcg = then_else \<open>rule is_complex_goal\<close> \<open>fail\<close> 
-  \<open>find_goal \<open>rule is_complex_goal\<close>, 
-  (rule is_complex_goal | tactic \<open>defer_tac 1\<close>)\<close>
-
-method sep_auto_all = (defer_vcg | (rule is_complex_goal, sep_auto))+
-
-lemma [sep_heap_rules]: "<tabinst_m_assn t t_m> 
-    Array.len (fst t_m) 
-    <\<lambda>r. tabinst_m_assn t t_m * \<up>(r=length (fst t))>"
-  unfolding tabinst_m_assn_def
-  by (sep_auto split: prod.splits)
-
-lemma [sep_heap_rules]: "<tabinst_m_assn t t_m> 
-    Array.nth (fst t_m) x
-    <\<lambda>r. tabinst_m_assn t t_m * \<up>(r=(fst t)!x)>"
-  unfolding tabinst_m_assn_def
-  by (sep_auto split: prod.splits)
-
-lemma funcs_nth_type_triple:"<funcs_m_assn i_s cls cls_m> 
-    Array.nth cls_m i  
-    <\<lambda>r. \<up>(cl_m_type r = cl_type (cls!i)) * funcs_m_assn i_s cls cls_m>" 
-  unfolding funcs_m_assn_def list_assn_conv_idx
-  apply(sep_auto heap del:nth_rule)
-  apply(extract_pre_pure)
-  apply(sep_auto)
-  apply(simp add: listI_assn_extract[of i])
-  using cl_m_assn_type 
-  by (metis mod_starD)
 
 lemma call_indirect_triple:
   assumes "inst_at (is, i_ms) (f_inst f, f_inst2) j"
@@ -464,22 +496,346 @@ lemma call_indirect_triple:
   done
 
 
-find_theorems app_s_f_v_s_mem_size
 
-lemmas splits = 
-  frame_context_m.splits frame_context.splits config.splits config_m.splits redex.splits prod.splits
 
-lemmas defs =  
-  Heap_Monad.return_def Heap_Monad.heap_def 
-  config_m_to_config_def frame_context_m_to_frame_context_def
+(* memory stuff *)
 
+lemma [sep_heap_rules]: 
+    "< mem_m_assn m m_m > 
+      grow_zeroed_byte_array (fst m_m) n 
+    <\<lambda>r. mem_m_assn (mem_append m n 0) (r,snd m_m)>\<^sub>t"
+  unfolding mem_m_assn_def mem_append_def mem_rep_append_def
+  by(sep_auto split:prod.splits simp:Abs_mem_rep_inverse)
+
+lemma mem_grow_triple:
+  assumes "inst_at (is, i_ms) (f_inst f, f_inst2) j" 
+  shows 
+  "< mems_m_assn ms ms_m * inst_store_assn (is, i_ms) > 
+    app_s_f_v_s_mem_grow_m ms_m f_inst2 v_s 
+  <\<lambda>r. let (ms', v_s', res) = app_s_f_v_s_mem_grow ms f v_s in
+   \<up>(r = (v_s', res)) * mems_m_assn ms' ms_m * inst_store_assn (is, i_ms)>\<^sub>t"
+proof - 
+  note expand = smem_ind_def mem_grow_def Let_def mem_size_def mem_length_def
+        mem_rep_length_def mem_max_def
+  note expand_with_assn = expand mem_m_assn_def mem_append_def
+  note splits = option.splits list.splits if_splits prod.splits
+
+  (* the "sep_auto simp:expand split:splits" list eliminate subgoals 
+    by finding contradictions in their assumptions *)
+  show ?thesis
+    using assms 
+    unfolding app_s_f_v_s_mem_grow_m_def app_s_f_v_s_mem_grow_def 
+      inst_m_assn_def mems_m_assn_def
+      list_assn_conv_idx
+    apply(sep_auto split: v.splits)
+        apply(knock_down "j")
+       apply(sep_auto)
+        apply(extract_list_idx "inst.mems (f_inst f) ! 0") 
+        (* not reinserting immediately -- the extracted mem_m_assn keeps being necessary *)
+        apply(sep_auto) 
+       apply(sep_auto simp:expand split:splits) 
+          apply(rule listI_assn_reinsert_upd, frame_inference, simp, simp)
+          apply(sep_auto simp:mem_append_def zero_byte_def)
+         apply(sep_auto simp:expand_with_assn split:splits)
+        apply(sep_auto)
+         apply(sep_auto simp:expand_with_assn split:splits) 
+        apply(sep_auto simp:expand_with_assn split:splits) 
+       apply(rule listI_assn_reinsert', frame_inference, simp, simp)
+       apply(sep_auto)
+      apply(sep_auto_all)
+    done
+qed
+
+named_theorems load_rules
+
+abbreviation "load32_mem_triple fl sx t_len m m_m n \<equiv> 
+   <mem_m_assn m m_m> 
+  fl (fst m_m) n         
+   <\<lambda>r. \<up>(i32_impl_abs r = (deserialise_i32 \<circ> (case sx of S \<Rightarrow> sign_extend S 4 | U \<Rightarrow> id)) 
+  (read_bytes m n t_len) 
+  \<and> n + t_len \<le> mem_length m) 
+  * mem_m_assn m m_m>" 
+
+lemma [load_rules]: 
+  "load32_mem_triple load_uint32           U 4 m m_m n"
+  "load32_mem_triple load_uint32_of_uint8  U 1 m m_m n"
+  "load32_mem_triple load_uint32_of_sint8  S 1 m m_m n"
+  "load32_mem_triple load_uint32_of_uint16 U 2 m m_m n"
+  "load32_mem_triple load_uint32_of_sint16 S 2 m m_m n"
+  unfolding mem_m_assn_def i32_impl_abs_def deserialise_i32_def
+    read_bytes_def mem_rep_read_bytes_def t_length_def mem_length_def mem_rep_length_def
+  by (sep_auto simp:Abs_uint32'.rep_eq word_list_sign_extend_Rep_uint8 split:prod.splits)+
+
+abbreviation "load64_mem_triple fl sx t_len m m_m n \<equiv> 
+   <mem_m_assn m m_m> 
+  fl (fst m_m) n         
+   <\<lambda>r. \<up>(i64_impl_abs r = (deserialise_i64 \<circ> (case sx of S \<Rightarrow> sign_extend S 8 | U \<Rightarrow> id)) 
+  (read_bytes m n t_len) 
+  \<and> n + t_len \<le> mem_length m) 
+  * mem_m_assn m m_m>" 
+
+lemma [load_rules]: 
+  "load64_mem_triple load_uint64           U 8 m m_m n"
+  "load64_mem_triple load_uint64_of_uint8  U 1 m m_m n"
+  "load64_mem_triple load_uint64_of_sint8  S 1 m m_m n"
+  "load64_mem_triple load_uint64_of_uint16 U 2 m m_m n"
+  "load64_mem_triple load_uint64_of_sint16 S 2 m m_m n"
+  "load64_mem_triple load_uint64_of_uint32 U 4 m m_m n"
+  "load64_mem_triple load_uint64_of_sint32 S 4 m m_m n"
+  unfolding mem_m_assn_def i64_impl_abs_def deserialise_i64_def
+    read_bytes_def mem_rep_read_bytes_def t_length_def mem_length_def mem_rep_length_def
+  by (sep_auto simp:Abs_uint64'.rep_eq word_list_sign_extend_Rep_uint8 split:prod.splits)+
+
+
+lemma load_triple: 
+  "<mem_m_assn m m_m>
+  load_m_v m_m n off t
+  <\<lambda>r_opt. expect_assn (\<lambda>r r_m. \<up>(r_m = wasm_deserialise r t)) true 
+  (load m n off (t_length t)) r_opt
+  * mem_m_assn m m_m>"
+  unfolding load_m_v_def load_def wasm_deserialise_def 
+  by(sep_auto heap:load_rules split:t.splits simp:mem_length_def mem_rep_length_def
+      read_bytes_def mem_rep_read_bytes_def t_length_def 
+serialise_deserialise_i32 serialise_deserialise_i64)
+
+
+
+lemma sign_extend_id: 
+  "sign_extend sx (length bs) bs = bs"
+  unfolding sign_extend_def
+  by(simp add:msb_byte_def msbyte_def bytes_takefill_def)
+
+lemma read_bytes_length:"n+l \<le> mem_length m \<Longrightarrow> length (read_bytes m n l) = l" 
+  unfolding mem_length_def mem_rep_length_def read_bytes_def mem_rep_read_bytes_def
+  by simp
+
+lemma deserialise_i32_absorb_sign_extend: 
+  "length bs \<le> 4 \<Longrightarrow> deserialise_i32 (sign_extend U 4 bs) = deserialise_i32 bs"
+  unfolding deserialise_i32_def word_rcat_rev_def sign_extend_def bytes_takefill_def
+    takefill_def zero_byte_def
+  apply(simp split:list.splits)
+  apply(auto)
+     apply (simp add: zero_uint8.rep_eq)+
+  done
+
+lemma deserialise_i64_absorb_sign_extend: 
+  "length bs \<le> 8 \<Longrightarrow> deserialise_i64 (sign_extend U 8 bs) = deserialise_i64 bs"
+  unfolding deserialise_i64_def word_rcat_rev_def sign_extend_def bytes_takefill_def
+    takefill_def zero_byte_def
+  apply(simp split:list.splits)
+  apply(auto)
+     apply (simp add: zero_uint8.rep_eq)+
+  done
+
+lemma [load_rules]:
+ "<mem_m_assn m m_m> 
+  load_uint32_packed (fst m_m) n tp sx        
+   <\<lambda>r. \<up>(i32_impl_abs r = (deserialise_i32 \<circ> sign_extend sx 4) (read_bytes m n (tp_length tp)) 
+  \<and> n + 1 \<le> mem_length m) 
+  * mem_m_assn m m_m>"
+  unfolding load_uint32_packed_def 
+  supply [simp] = tp_length_def t_length_def
+  apply(sep_auto split:tp.splits sx.splits)
+       apply(sep_auto heap:load_rules)+
+  subgoal  using read_bytes_length sign_extend_id
+    by metis
+    apply(sep_auto heap:load_rules, 
+      simp add:read_bytes_length deserialise_i32_absorb_sign_extend )+
+  done 
+
+lemma [load_rules]:
+ "<mem_m_assn m m_m> 
+  load_uint64_packed (fst m_m) n tp sx        
+   <\<lambda>r. \<up>(i64_impl_abs r = (deserialise_i64 \<circ> sign_extend sx 8) (read_bytes m n (tp_length tp)) 
+  \<and> n + 1 \<le> mem_length m) 
+  * mem_m_assn m m_m>"
+  unfolding load_uint64_packed_def 
+  supply [simp] = tp_length_def t_length_def
+  apply(sep_auto split:tp.splits sx.splits)
+       apply(sep_auto heap:load_rules, 
+        (simp add:read_bytes_length deserialise_i64_absorb_sign_extend)?)+
+  done 
+
+(* Note to self: had issues with sep_auto instantiating the postcondition by dropping the pure precondition *)
+
+lemma load_packed_triple: 
+  "<mem_m_assn m m_m>
+  load_packed_m_v m_m n off t tp sx
+  <\<lambda>r_opt. expect_assn (\<lambda>r r_m. \<up>(r_m = wasm_deserialise r t)) true
+      (load_packed sx m n off (tp_length tp) (t_length t)) r_opt
+  * mem_m_assn m m_m>"
+  unfolding load_packed_m_v_def load_packed_def 
+  supply [simp] = t_length_def load_def wasm_deserialise_def mem_length_def mem_rep_length_def
+    and [sep_heap_rules] = load_rules
+    and [split] = option.splits t.splits
+  apply(sep_auto)
+     apply(sep_auto simp: sign_extend_def bytes_takefill_def serialise_deserialise_i32) 
+    apply(sep_auto)
+   apply(sep_auto simp: sign_extend_def bytes_takefill_def serialise_deserialise_i64) 
+   apply(sep_auto)
+  done
+
+lemma load_maybe_packed_triple:
+  assumes "inst_at (is, i_ms) (f_inst f, f_inst2) j"
+  shows "<mems_m_assn ms ms_m * inst_store_assn (is, i_ms)>
+  app_s_f_v_s_load_maybe_packed_m t tp_sx off ms_m f_inst2 v_s
+  <\<lambda>r.\<up>(r = app_s_f_v_s_load_maybe_packed t tp_sx off ms f v_s)
+  * mems_m_assn ms ms_m * inst_store_assn (is, i_ms)>\<^sub>t"
+proof -
+  note expand = smem_ind_def Let_def mem_size_def mem_length_def
+        mem_rep_length_def mem_max_def
+  note splits = option.splits list.splits if_splits prod.splits
+
+  show ?thesis
+    using assms 
+    unfolding app_s_f_v_s_load_maybe_packed_m_def app_s_f_v_s_load_maybe_packed_def 
+      app_s_f_v_s_load_packed_def app_s_f_v_s_load_def
+      inst_m_assn_def mems_m_assn_def
+      list_assn_conv_idx
+    supply [sep_heap_rules] = load_triple load_packed_triple
+    apply(sep_auto split:v.splits)
+     apply(sep_auto split:option.splits)
+    apply(sep_auto split:v.splits)
+        apply(knock_down j)
+       apply(sep_auto split:option.splits)    
+               apply(sep_auto?, knock_down "inst.mems (f_inst f) ! 0",
+        sep_auto simp:expand split:splits)+ (*takes a moment*)   
+      apply(sep_auto split:splits)+
+    done
+qed
+
+
+named_theorems store_rules
+
+abbreviation "store32_mem_triple fs t_len m m_m n v \<equiv> 
+   <mem_m_assn m m_m> 
+  fs (fst m_m) n (i32_impl_rep v)
+   <\<lambda>r. \<up>(n + t_len \<le> mem_length m) 
+  * mem_m_assn (write_bytes m n (bytes_takefill zero_byte t_len (serialise_i32 v))) m_m>" 
+
+lemma [store_rules]:
+  "store32_mem_triple store_uint32           4 m m_m n v"
+  "store32_mem_triple store_uint8_of_uint32  1 m m_m n v"
+  "store32_mem_triple store_uint16_of_uint32 2 m m_m n v"
+  unfolding mem_m_assn_def 
+  by(sep_auto split:prod.splits 
+      simp:write_bytes_def mem_rep_write_bytes_def mem_length_def mem_rep_length_def
+      Abs_mem_rep_inverse serialise_i32_def word_rsplit_rev_def 
+      i32_impl_rep.rep_eq bytes_takefill_def numeral_Bit0)+
+
+abbreviation "store64_mem_triple fs t_len m m_m n v \<equiv> 
+   <mem_m_assn m m_m> 
+  fs (fst m_m) n (i64_impl_rep v)
+   <\<lambda>r. \<up>(n + t_len \<le> mem_length m) 
+  * mem_m_assn (write_bytes m n (bytes_takefill zero_byte t_len (serialise_i64 v))) m_m>" 
+
+lemma [store_rules]:
+  "store64_mem_triple store_uint64           8 m m_m n v"
+  "store64_mem_triple store_uint8_of_uint64  1 m m_m n v"
+  "store64_mem_triple store_uint16_of_uint64 2 m m_m n v"
+  "store64_mem_triple store_uint32_of_uint64 4 m m_m n v"
+  unfolding mem_m_assn_def 
+  by(sep_auto split:prod.splits 
+      simp:write_bytes_def mem_rep_write_bytes_def mem_length_def mem_rep_length_def
+      Abs_mem_rep_inverse serialise_i64_def word_rsplit_rev_def 
+      i64_impl_rep.rep_eq bytes_takefill_def numeral_Bit0)+
+
+lemma store_triple: 
+  "<mem_m_assn m m_m>
+  store_m_v m_m n off v
+  <\<lambda>r_opt. expect_assn (\<lambda>m' r_m. mem_m_assn m' m_m) (mem_m_assn m m_m)
+    (store m n off (bits v) (t_length (typeof v))) r_opt>"
+  unfolding store_m_v_def
+  apply(sep_auto split:v.splits heap:store_rules 
+      simp: serialise_deserialise_i32 serialise_f32_len 
+      serialise_deserialise_i64 serialise_f64_len 
+      store_def bits_def t_length_def typeof_def mem_length_def mem_rep_length_def)
+  done
+
+lemma [store_rules]:
+ "<mem_m_assn m m_m> 
+  store_uint32_packed (fst m_m) n (i32_impl_rep v) tp
+   <\<lambda>r.\<up>(n + (tp_length tp) \<le> mem_length m) * 
+   mem_m_assn (write_bytes m n (bytes_takefill zero_byte (tp_length tp) (serialise_i32 v))) m_m >"
+  unfolding store_uint32_packed_def 
+  by(sep_auto simp:tp_length_def split:tp.splits heap:store_rules)
+
+lemma [store_rules]:
+ "<mem_m_assn m m_m> 
+  store_uint64_packed (fst m_m) n (i64_impl_rep v) tp
+   <\<lambda>r. \<up>(n + (tp_length tp) \<le> mem_length m) *
+   mem_m_assn  (write_bytes m n (bytes_takefill zero_byte (tp_length tp) (serialise_i64 v))) m_m >"
+  unfolding store_uint64_packed_def 
+  by(sep_auto simp:tp_length_def split:tp.splits heap:store_rules)
+
+lemma store_packed_triple: 
+  "<mem_m_assn m m_m>
+  store_packed_m_v m_m n off v tp
+  <\<lambda>r_opt. expect_assn (\<lambda>m' r_m. mem_m_assn m' m_m) (mem_m_assn m m_m)
+    (store_packed m n off (bits v) (tp_length tp)) r_opt>" 
+  unfolding store_packed_m_v_def 
+  by (sep_auto split:v.splits heap:store_rules 
+      simp:store_packed_def store_def bits_def
+      mem_length_def mem_rep_length_def 
+      serialise_deserialise_i32 serialise_f32_len
+      serialise_deserialise_i64 serialise_f64_len)
+  
+
+lemma store_maybe_packed_triple:
+  assumes "inst_at (is, i_ms) (f_inst f, f_inst2) j"
+  shows "<mems_m_assn ms ms_m * inst_store_assn (is, i_ms)>
+  app_s_f_v_s_store_maybe_packed_m t tp_sx off ms_m f_inst2 v_s
+  <\<lambda>r. let (ms', v_s', res) = app_s_f_v_s_store_maybe_packed t tp_sx off ms f v_s in 
+  \<up>(r = (v_s', res))
+  * mems_m_assn ms' ms_m * inst_store_assn (is, i_ms)>\<^sub>t" 
+proof -
+  note expand = smem_ind_def mem_grow_def Let_def mem_size_def mem_length_def
+        mem_rep_length_def mem_max_def types_agree_def
+  note splits = option.splits list.splits if_splits prod.splits
+
+  show ?thesis
+    using assms
+    unfolding 
+      app_s_f_v_s_store_maybe_packed_m_def app_s_f_v_s_store_maybe_packed_def
+      app_s_f_v_s_store_def app_s_f_v_s_store_packed_def
+      inst_m_assn_def mems_m_assn_def
+      list_assn_conv_idx
+    apply(sep_auto)
+     apply(sep_auto split:option.splits prod.splits simp:app_s_f_v_s_store_packed_def) 
+    apply(sep_auto split:list.splits)
+     apply(sep_auto split:option.splits prod.splits simp:app_s_f_v_s_store_packed_def)
+    apply(sep_auto split:v.splits)
+
+         apply(knock_down j)
+        apply(cases tp_sx) 
+         apply(sep_auto)
+          apply(extract_list_idx "inst.mems (f_inst f) ! 0")
+          apply(sep_auto heap:store_triple)
+         apply(sep_auto simp:expand split:splits)
+          apply(rule listI_assn_reinsert, frame_inference, simp, simp, sep_auto)
+         apply(sep_auto simp:expand split:splits)
+         apply(rule listI_assn_reinsert_upd, frame_inference, simp, simp, sep_auto)
+
+        apply(sep_auto)
+          apply(extract_list_idx "inst.mems (f_inst f) ! 0")
+          apply(sep_auto heap:store_packed_triple)
+         apply(sep_auto simp:expand split:splits)
+          apply(rule listI_assn_reinsert, frame_inference, simp, simp, sep_auto)
+         apply(sep_auto simp:expand split:splits)
+        apply(rule listI_assn_reinsert_upd, frame_inference, simp, simp, sep_auto)
+       apply(sep_auto simp:expand split:splits)+
+    done
+qed
+
+
+
+(* run_step_b_e *)
 
 abbreviation cfg_m_pair_assn where 
   "cfg_m_pair_assn i_s p p_m \<equiv> 
   let (cfg, res) = p in 
   let (cfg_m, res_m) = p_m in 
   cfg_m_assn i_s cfg cfg_m * \<up>(res = res_m)"
-
   
 lemma run_step_b_e_m_triple:
     "<cfg_m_assn i_s cfg cfg_m> 
@@ -502,61 +858,57 @@ proof -
     by(erule redex.exhaust)
 
   note unfold_vars_m = config_m frame_m redex_m
-
   note unfold_vars = config frame redex unfold_vars_m
-
   note unfold_vars_assns = unfold_vars cfg_m_assn_def fc_m_assn_def
 
   show ?thesis
   proof (cases b_e)
-    case (Tee_local k)
-    then show ?thesis unfolding unfold_vars_assns by sep_auto
+    case (Get_global k)
+    then show ?thesis unfolding unfold_vars_assns s_m_assn_def 
+      by (sep_auto heap:get_global_triple split:prod.splits)
   next
     case (Set_global k)
     then show ?thesis unfolding unfold_vars_assns s_m_assn_def 
-      (*comment on instability*)
       by (sep_auto heap:set_global_triple split:prod.splits)
   next
     case (Load t tp_sx a off)
-    then show ?thesis sorry
+    then show ?thesis unfolding unfold_vars_assns s_m_assn_def 
+      by (sep_auto heap:load_maybe_packed_triple split:prod.splits)
   next
     case (Store t tp a off)
-    then show ?thesis sorry
+    then show ?thesis unfolding unfold_vars_assns s_m_assn_def
+      by (sep_auto heap:store_maybe_packed_triple split:prod.splits)
   next
     case Grow_memory
-    then show ?thesis sorry
+    then show ?thesis unfolding unfold_vars_assns s_m_assn_def 
+      by (sep_auto heap:mem_grow_triple split:prod.splits)
   next
     case Current_memory
-    then show ?thesis 
-      unfolding unfold_vars_assns s_m_assn_def mems_m_assn_def 
-      by(sep_auto heap:mem_size_triple split:prod.splits)
-  next
-    case (Set_local k)
-    then show ?thesis 
-      unfolding unfold_vars_assns
-      by (sep_auto heap: set_local_triple[of _ _ f f_inst2] split:prod.splits)
+    then show ?thesis unfolding unfold_vars_assns s_m_assn_def 
+      by (sep_auto heap:mem_size_triple split:prod.splits)
   next
     case (Get_local k)
     then show ?thesis 
       unfolding unfold_vars_assns by (sep_auto heap:get_local_triple)
   next
-    case (Get_global k)
-    then show ?thesis 
-      unfolding unfold_vars_assns s_m_assn_def by (sep_auto heap:get_global_triple split:prod.splits)
+    case (Set_local k)
+    then show ?thesis unfolding unfold_vars_assns
+      by (sep_auto heap: set_local_triple split:prod.splits)
+  next
+    case (Tee_local k)
+    then show ?thesis unfolding unfold_vars_assns by sep_auto
   next
     case (Call k)
-    then show ?thesis 
-      unfolding unfold_vars_assns by (sep_auto heap:call_triple split:prod.splits)
+    then show ?thesis unfolding unfold_vars_assns 
+      by (sep_auto heap:call_triple split:prod.splits)
   next
     case (Call_indirect k)
-    then show ?thesis 
-      unfolding unfold_vars_assns s_m_assn_def by (sep_auto heap:call_indirect_triple split:prod.splits)
+    then show ?thesis unfolding unfold_vars_assns s_m_assn_def 
+      by (sep_auto heap:call_indirect_triple split:prod.splits)
   next
-    case Return (* this case relies on garbage collection *)
-
-    show ?thesis
-      unfolding Return unfold_vars_assns fcs_m_assn_def
-      by (sep_auto split:splits list.split)
+    case Return 
+    then show ?thesis unfolding unfold_vars_assns fcs_m_assn_def
+      by (sep_auto split:frame_context_m.splits frame_context.splits list.split)
   next
     case (Block tf b_ebs)
     then show ?thesis unfolding unfold_vars_assns by(sep_auto split:tf.splits)
@@ -608,67 +960,39 @@ proof -
   qed
 qed
 
-abbreviation "s_m_vs_pair_assn i_s \<equiv> \<lambda>(s, vs) (s_m, vs_m). s_m_assn i_s s s_m * \<up>(vs=vs_m)"
 
-abbreviation "s_m_vs_opt_assn i_s a a_m s s_m \<equiv> (case a of 
-   Some s_vs \<Rightarrow> (case a_m of Some s_vs_m \<Rightarrow> s_m_vs_pair_assn i_s s_vs s_vs_m | None \<Rightarrow> false) 
- | None \<Rightarrow> (case a_m of Some s_vs_m \<Rightarrow> false | None \<Rightarrow> s_m_assn i_s s s_m)) "
+(* run_step_e_m *)
+
+abbreviation "s_m_vs_pair_assn i_s \<equiv> \<lambda>(s, vs) (s_m, vs_m). s_m_assn i_s s s_m * \<up>(vs=vs_m)"
 
 lemma host_apply_impl_m_triple:
  "< s_m_assn i_s s s_m>
  host_apply_impl_m s_m tf h vs
- <\<lambda>r. s_m_vs_opt_assn i_s (host_apply_impl s tf h vs) r s s_m>"
+ <\<lambda>r_opt. expect_assn (\<lambda>r r_m. s_m_vs_pair_assn i_s r r_m) (s_m_assn i_s s s_m)
+  (host_apply_impl s tf h vs) r_opt >"
   sorry
 
-lemma host_apply_impl_m_triple':
- "< funcs_m_assn i_s (s.funcs s) (s_m.funcs s_m) 
-* tabs_m_assn (s.tabs s) (s_m.tabs s_m) * mems_m_assn (s.mems s) (s_m.mems s_m) 
-* globs_m_assn (s.globs s) (s_m.globs s_m)>
- host_apply_impl_m s_m tf h vs
- <\<lambda>r. s_m_vs_opt_assn i_s (host_apply_impl s tf h vs) r s s_m>"
-  sorry
-
-lemma host_apply_impl_m_triple'':
- "< s_m.funcs s_m \<mapsto>\<^sub>a fs_i * list_assn (cl_m_assn i_s) (s.funcs s) fs_i
-* tabs_m_assn (s.tabs s) (s_m.tabs s_m) * mems_m_assn (s.mems s) (s_m.mems s_m) 
-* globs_m_assn (s.globs s) (s_m.globs s_m)>
- host_apply_impl_m s_m tf h vs
- <\<lambda>r. s_m_vs_opt_assn i_s (host_apply_impl s tf h vs) r s s_m>"
-  sorry
-
-
-lemma ent_triple_preI:
-  assumes "\<And>h. h\<Turnstile>P \<Longrightarrow> P \<Longrightarrow>\<^sub>A Q"
-  shows "P \<Longrightarrow>\<^sub>A Q"
-  using assms unfolding entails_def by auto
-
-method extract_pre_pure' uses dest =
-  (rule hoare_triple_preI | rule ent_triple_preI | drule asm_rl[of "_\<Turnstile>_"]),
-  (determ \<open>elim mod_starE dest[elim_format] extract_pure_rules[elim_format]\<close>)?,
-  ((determ \<open>thin_tac "_ \<Turnstile> _"\<close>)+)?,
-  (simp (no_asm) only: triv_forall_equality)?
-
-lemma pure_dup:
-  assumes "is_pure_assn P" 
-  shows "P = P*P" 
-  using assms unfolding is_pure_assn_def
-  by auto
-
-
-lemma [sep_heap_rules]:
+lemma funcs_nth_triple:
   "< fs_m\<mapsto>\<^sub>a fs_i * list_assn (cl_m_assn i_s) fs fs_i> 
   Array.nth fs_m i 
   <\<lambda>r. \<up>(i < length fs_i \<and> r = fs_i!i) 
   * cl_m_assn i_s (fs!i) r * fs_m \<mapsto>\<^sub>a fs_i * list_assn (cl_m_assn i_s) fs fs_i>"
   unfolding funcs_m_assn_def list_assn_conv_idx 
   apply(sep_auto)
-  apply(extract_pre_pure')
+  apply(extract_pre_pure)
   apply(extract_list_idx i)
   apply(subst pure_dup[OF cl_m_assn_pure])
   apply(reinsert_list_idx i)
   apply(sep_auto)
   done
 
+lemma funcs_nth_triple_s:
+  "< s_m_assn i_s s s_m> 
+  Array.nth (s_m.funcs s_m) i 
+  <\<lambda>r. \<up>(i < length (s.funcs s)) 
+  * cl_m_assn i_s (s.funcs s!i) r * s_m_assn i_s s s_m>"
+  unfolding s_m_assn_def funcs_m_assn_def
+  by (sep_auto heap:funcs_nth_triple heap del:nth_rule, extract_pre_pure)
 
 lemma run_step_e_m_triple:
     "<cfg_m_assn i_s cfg cfg_m> 
@@ -704,13 +1028,12 @@ proof -
     case (Invoke i_cl)
 
     show ?thesis unfolding Invoke unfold_vars_assns 
+      apply(sep_auto heap: funcs_nth_triple_s split:cl_m.splits) 
       supply [simp] = Let_def and 
-        [split] = splits v.splits option.splits cl.splits cl_m.splits tf.splits nat.splits
-      and [sep_heap_rules] = host_apply_impl_m_triple''
-      apply(sep_auto simp:s_m_assn_def funcs_m_assn_def heap del: nth_rule)
-      supply [simp] = cl_m_assn_def locs_m_assn_def s_m_assn_def funcs_m_assn_def fc_m_assn_def 
-                apply(sep_auto_all)
-      apply (sep_auto)
+        [split] = v.splits option.splits 
+        cl.splits cl_m.splits tf.splits nat.splits
+       apply(sep_auto simp:cl_m_assn_def locs_m_assn_def s_m_assn_def funcs_m_assn_def fc_m_assn_def)
+      apply(sep_auto heap:host_apply_impl_m_triple simp:cl_m_assn_def)
       done
   next
     case Trap
@@ -724,42 +1047,79 @@ proof -
   qed
 qed 
 
-lemma run_step_e_m_run_step_e:
-  assumes 
-    "execute (run_step_e_m e cfg_m) h = Some ((cfg_m', res), h')"
-  shows 
-    "run_step_e e (config_m_to_config h cfg_m) = ((config_m_to_config h' cfg_m'), res)"
-proof(cases e)
-  case (Basic b_e)
-  have 1:"run_step_e_m e cfg_m = run_step_b_e_m b_e cfg_m" unfolding Basic
-    by(rule config_m.induct, auto simp add: defs split: splits)
-  have "run_step_e e (config_m_to_config h cfg_m) = run_step_b_e b_e (config_m_to_config h cfg_m)"
-    unfolding Basic by(rule config.induct, auto simp add: defs split: splits) 
-  also have "... = ((config_m_to_config h' cfg_m'), res)" 
-    using assms sorry
-  finally show ?thesis by -
-next
-  case (Invoke i_cl)
-  then show ?thesis sorry
-next
-  case Trap
-  show ?thesis using assms by (auto simp add: defs Trap split: splits)
-next
-  case (Label x41 x42 x43)
-  show ?thesis using assms by (auto simp add: defs Label split: splits)
-next
-  case (Frame x51 x52 x53)
-  show ?thesis using assms by (auto simp add: defs Frame split: splits)
-qed
 
-lemma run_iter_m_run_iter:
-  "execute (run_iter_m n cfg_m) h = Some ((cfg_m', res), h')
- \<Longrightarrow> run_iter n (config_m_to_config h cfg_m) = ((config_m_to_config h' cfg_m'), res)"
-proof(induct n)
+(* run_iter *)
+
+lemma update_fc_return_preserve_assn:
+  "cfg_m_assn i_s (Config d s fc (fc'#fcs)) (Config_m d_m s_m fc_m (fc'_m#fcs_m)) 
+  \<Longrightarrow>\<^sub>A cfg_m_assn i_s (Config (Suc d) s (update_fc_return fc' v_s) fcs)
+    (Config_m (Suc d_m) s_m (update_fc_return_m fc'_m v_s) fcs_m) * true"
+  unfolding cfg_m_assn_def 
+  apply (sep_auto)
+  unfolding fc_m_assn_def
+  by (sep_auto split:frame_context.splits frame_context_m.splits)
+
+lemma update_redex_lc_preserve_assn:"cfg_m_assn i_s 
+       (Config d s (Frame_context redex lcs nf f) fcs)
+       (Config_m d_m s_m (Frame_context_m redex_m 
+        lcs_m nf_m f_locs1 f_inst2) fcs_m)
+  \<Longrightarrow>\<^sub>A cfg_m_assn i_s 
+       (Config d s (Frame_context (g1 redex lcs) (g2 redex lcs) nf f) fcs)
+       (Config_m d_m s_m (Frame_context_m (g1 redex_m lcs) 
+        (g2 redex_m lcs_m) nf_m f_locs1 f_inst2) fcs_m) "
+  unfolding cfg_m_assn_def fc_m_assn_def
+  by (sep_auto)
+
+lemma run_iter_m_triple:
+    "<cfg_m_assn i_s cfg cfg_m> 
+    run_iter_m n cfg_m 
+    <\<lambda>r. cfg_m_pair_assn i_s (run_iter n cfg) r>\<^sub>t"
+proof(induct n arbitrary: i_s cfg cfg_m)
   case 0
-  show ?case using 0 by (auto simp add: defs split: splits)
+  show ?case unfolding 0 by sep_auto
 next
   case (Suc n)
-  then show ?case sorry
+
+  obtain d s fc fcs where config:"cfg = Config d s fc fcs"
+    by(erule config.exhaust)
+  obtain redex lcs nf f where frame:"fc = Frame_context redex lcs nf f" 
+    by(erule frame_context.exhaust)
+  obtain v_s es b_es where redex:"redex = Redex v_s es b_es" 
+    by(erule redex.exhaust)
+  obtain d_m s_m fc_m fcs_m where config_m:"cfg_m = Config_m d_m s_m fc_m fcs_m" 
+    by(erule config_m.exhaust)  
+  obtain redex_m lcs_m nf_m f_locs1 f_inst2 
+    where frame_m:"fc_m = Frame_context_m redex_m lcs_m nf_m f_locs1 f_inst2" 
+    by(erule frame_context_m.exhaust)
+  obtain v_s_m es_m b_es_m where redex_m:"redex_m = Redex v_s_m es_m b_es_m" 
+    by(erule redex.exhaust)
+  note unfold_vars_m = config_m frame_m redex_m
+  note unfold_vars = config frame redex unfold_vars_m
+
+  show ?case unfolding unfold_vars
+    supply [simp del] = run_step_b_e_m.simps run_step_b_e.simps 
+      run_step_e_m.simps run_step_e.simps
+    apply(extract_pre_pure, simp add:cfg_m_assn_pure_def fc_m_assn_pure_def)
+    apply(sep_auto)
+       apply(cases fcs, auto)
+       apply(rule cons_pre_rule[OF update_fc_return_preserve_assn])
+       apply(sep_auto heap:Suc)
+      apply(sep_auto split:label_context.splits)
+      apply(rule cons_pre_rule[OF update_redex_lc_preserve_assn])
+      apply(sep_auto heap:Suc)
+     apply(sep_auto split:prod.splits)
+      apply(rule cons_pre_rule[OF update_redex_lc_preserve_assn])
+      apply(sep_auto heap:Suc)
+     apply(sep_auto)
+      apply(rule cons_pre_rule[OF update_redex_lc_preserve_assn])
+      apply(sep_auto heap:run_step_b_e_m_triple)
+     apply(sep_auto split:prod.splits res_step.splits heap:Suc)
+    apply(sep_auto)
+     apply(rule cons_pre_rule[OF update_redex_lc_preserve_assn])
+     apply(sep_auto heap:run_step_e_m_triple)
+    apply(sep_auto split:res_step.splits prod.splits heap:Suc)
+    done
 qed
+
+
 end
