libs/Byte_Array.thy
@@ -248,4 +248,169 @@ definition store_uint32_of_uint64 :: "byte_array \<Rightarrow> nat \<Rightarrow>
 definition store_uint64 :: "byte_array \<Rightarrow> nat \<Rightarrow> uint64 \<Rightarrow> unit Heap" where
   "store_uint64 a n v \<equiv> store_uintX_of_uint64 a n v 8"
 
+(* load/store heap rules *) 
+
+lemma [sep_heap_rules]: "<a \<mapsto>\<^sub>b\<^sub>a la> 
+  load_uint8 a n
+   <\<lambda>r. \<up>(n < length la \<and> r = la!n) * a \<mapsto>\<^sub>b\<^sub>a la >"
+  unfolding load_uint8_def bl_assn_def 
+  by sep_auto
+
+lemma [sep_heap_rules]: "<a \<mapsto>\<^sub>b\<^sub>a la> 
+  store_uint8 a n b
+   <\<lambda>r. \<up>(n < length la) * a \<mapsto>\<^sub>b\<^sub>a la[n := b]>"
+  unfolding store_uint8_def bl_assn_def 
+  by sep_auto
+
+lemma [sep_heap_rules]: "<a \<mapsto>\<^sub>b\<^sub>a la> 
+  load_uint8_list a n x
+   <\<lambda>r. \<up>((if x > 0 then n+x \<le> length la else True) \<and> r = take x (drop n la) )
+   * a \<mapsto>\<^sub>b\<^sub>a la >"
+proof(induct x arbitrary:la a n)
+case 0
+  then show ?case by(sep_auto)
+next
+  case (Suc x)
+  show ?case 
+    apply(sep_auto heap:Suc)
+    using less_imp_Suc_add apply force
+    by (metis Cons_nth_drop_Suc take_Suc_Cons)
+qed
+
+lemma [sep_heap_rules]: "<a \<mapsto>\<^sub>b\<^sub>a la> 
+  store_uint8_list a n bs
+   <\<lambda>r. \<up>(case bs of [] \<Rightarrow> True | x#xs \<Rightarrow> n+length bs \<le> length la )
+   * a \<mapsto>\<^sub>b\<^sub>a (take n la @ bs @ drop (n+length bs) la) >"
+proof(induct bs arbitrary:a la n)
+case Nil
+  then show ?case by sep_auto
+next
+  case (Cons a bs)
+  show ?case by (sep_auto heap:Cons split:list.splits simp: take_update_last)
+qed
+
+lemma [sep_heap_rules]: "<a \<mapsto>\<^sub>b\<^sub>a la> 
+  load_uint32_of_uintX a n x
+   <\<lambda>r. \<up>(r = (Abs_uint32' \<circ> word_rcat_rev \<circ> map Rep_uint8') (take x (drop n la)) 
+ \<and> (if x > 0 then n+x \<le> length la else True)) * a \<mapsto>\<^sub>b\<^sub>a la >"
+  unfolding load_uint32_of_uintX_def by sep_auto
+
+lemma [sep_heap_rules]: "<a \<mapsto>\<^sub>b\<^sub>a la> 
+  load_uint32_of_sintX a n x
+   <\<lambda>r. \<up>(r = (Abs_uint32' \<circ> word_rcat_rev \<circ> word_list_sign_extend 4 \<circ> map Rep_uint8') 
+  (take x (drop n la)) 
+  \<and> (if x > 0 then n+x \<le> length la else True)) * a \<mapsto>\<^sub>b\<^sub>a la >"
+  unfolding load_uint32_of_sintX_def by sep_auto
+
+lemma [sep_heap_rules]: "<a \<mapsto>\<^sub>b\<^sub>a la> 
+  store_uintX_of_uint32 a n v x
+   <\<lambda>r. \<up>(if x > 0 then n+x \<le> length la else True)
+   * a \<mapsto>\<^sub>b\<^sub>a (take n la @ 
+    (map Abs_uint8' \<circ> takefill (0::8 word) x \<circ> word_rsplit_rev \<circ> Rep_uint32') v
+  @ drop (n+x) la) >"
+  unfolding store_uintX_of_uint32_def 
+  apply(sep_auto split:list.splits)
+   apply (metis length_takefill add.right_neutral add_Suc_right list.size(4)) 
+  apply(sep_auto)
+  done
+
+abbreviation "load32_triple fl sign t_len a la n \<equiv> 
+  <a \<mapsto>\<^sub>b\<^sub>a la> 
+  fl a n
+   <\<lambda>r. \<up>(r = (Abs_uint32' \<circ> word_rcat_rev \<circ> (if sign then word_list_sign_extend 4 else id) 
+   \<circ> map Rep_uint8') (take t_len (drop n la))
+  \<and> n+t_len \<le> length la) * a \<mapsto>\<^sub>b\<^sub>a la >" 
+
+lemma [sep_heap_rules]: 
+  "load32_triple load_uint32_of_uint8  False 1 a la n"
+  "load32_triple load_uint32_of_sint8  True  1 a la n"
+  "load32_triple load_uint32_of_uint16 False 2 a la n"
+  "load32_triple load_uint32_of_sint16 True  2 a la n"
+  "load32_triple load_uint32           False 4 a la n"
+  unfolding 
+    load_uint32_of_uint8_def load_uint32_of_sint8_def
+    load_uint32_of_uint16_def load_uint32_of_sint16_def
+    load_uint32_def
+  by sep_auto+
+
+abbreviation "store32_triple fs t_len a la n v \<equiv> 
+  <a \<mapsto>\<^sub>b\<^sub>a la> 
+  fs a n v 
+  <\<lambda>r. \<up>(n+t_len \<le> length la)
+   * a \<mapsto>\<^sub>b\<^sub>a (take n la @ 
+    (map Abs_uint8' \<circ> takefill (0::8 word) t_len \<circ> word_rsplit_rev \<circ> Rep_uint32') v
+  @ drop (n+t_len) la) >"
+
+lemma [sep_heap_rules]: 
+  "store32_triple store_uint8_of_uint32  1 a la n v"
+  "store32_triple store_uint16_of_uint32 2 a la n v"
+  "store32_triple store_uint32           4 a la n v"
+  unfolding store_uint8_of_uint32_def store_uint16_of_uint32_def store_uint32_def
+  by sep_auto+
+
+
+lemma [sep_heap_rules]: "<a \<mapsto>\<^sub>b\<^sub>a la> 
+  load_uint64_of_uintX a n x
+   <\<lambda>r. \<up>(r = (Abs_uint64' \<circ> word_rcat_rev \<circ> (map Rep_uint8')) (take x (drop n la)) 
+  \<and> (if x > 0 then n+x \<le> length la else True)) * a \<mapsto>\<^sub>b\<^sub>a la >"
+  unfolding load_uint64_of_uintX_def by sep_auto
+
+lemma [sep_heap_rules]: "<a \<mapsto>\<^sub>b\<^sub>a la> 
+  load_uint64_of_sintX a n x
+   <\<lambda>r. \<up>(r = (Abs_uint64' \<circ> word_rcat_rev \<circ> word_list_sign_extend 8 \<circ> map Rep_uint8') 
+  (take x (drop n la)) 
+  \<and> (if x > 0 then n+x \<le> length la else True)) * a \<mapsto>\<^sub>b\<^sub>a la >"
+  unfolding load_uint64_of_sintX_def by sep_auto
+
+lemma [sep_heap_rules]: "<a \<mapsto>\<^sub>b\<^sub>a la> 
+  store_uintX_of_uint64 a n v x
+   <\<lambda>r. \<up>(if x > 0 then n+x \<le> length la else True)
+   * a \<mapsto>\<^sub>b\<^sub>a (take n la @ 
+    (map Abs_uint8' \<circ> takefill (0::8 word) x \<circ> word_rsplit_rev \<circ> Rep_uint64') v
+  @ drop (n+x) la) >"
+  unfolding store_uintX_of_uint64_def 
+  apply(sep_auto split:list.splits)
+   apply (metis length_takefill add.right_neutral add_Suc_right list.size(4)) 
+  apply(sep_auto)
+  done
+
+abbreviation "load64_triple fl sign t_len a la n \<equiv> 
+  <a \<mapsto>\<^sub>b\<^sub>a la> 
+  fl a n
+   <\<lambda>r. \<up>(r = (Abs_uint64' \<circ> word_rcat_rev \<circ> (if sign then word_list_sign_extend 8 else id) 
+   \<circ> map Rep_uint8') (take t_len (drop n la))
+  \<and> n+t_len \<le> length la) * a \<mapsto>\<^sub>b\<^sub>a la >" 
+
+lemma [sep_heap_rules]: 
+  "load64_triple load_uint64_of_uint8  False 1 a la n"
+  "load64_triple load_uint64_of_sint8  True  1 a la n"
+  "load64_triple load_uint64_of_uint16 False 2 a la n"
+  "load64_triple load_uint64_of_sint16 True  2 a la n"
+  "load64_triple load_uint64_of_uint32 False 4 a la n"
+  "load64_triple load_uint64_of_sint32 True  4 a la n"
+  "load64_triple load_uint64           False 8 a la n"
+  unfolding 
+    load_uint64_of_uint8_def  load_uint64_of_sint8_def
+    load_uint64_of_uint16_def load_uint64_of_sint16_def
+    load_uint64_of_uint32_def load_uint64_of_sint32_def
+    load_uint64_def
+  by sep_auto+
+
+abbreviation "store64_triple fs t_len a la n v \<equiv> 
+  <a \<mapsto>\<^sub>b\<^sub>a la> 
+  fs a n v 
+  <\<lambda>r. \<up>(n+t_len \<le> length la)
+   * a \<mapsto>\<^sub>b\<^sub>a (take n la @ 
+    (map Abs_uint8' \<circ> takefill (0::8 word) t_len \<circ> word_rsplit_rev \<circ> Rep_uint64') v
+  @ drop (n+t_len) la) >"
+
+lemma [sep_heap_rules]: 
+  "store64_triple store_uint8_of_uint64  1 a la n v"
+  "store64_triple store_uint16_of_uint64 2 a la n v"
+  "store64_triple store_uint32_of_uint64 4 a la n v"
+  "store64_triple store_uint64           8 a la n v"
+  unfolding store_uint8_of_uint64_def store_uint16_of_uint64_def 
+            store_uint32_of_uint64_def store_uint64_def
+  by sep_auto+
+
 end
